veric/lifting_expr.v
@@ -71,6 +71,31 @@ Qed.
 
 Definition stack_level (n : nat) : assert := <affine> monPred_in(I := stack_index) n.
 
+Lemma stack_level_intro : ⊢ ∃ n, stack_level n.
+Proof.
+  by iDestruct (monPred_in_intro emp with "[]") as (?) "($ & _)".
+Qed.
+
+Lemma stack_level_elim : forall (P : assert) n, ⊢ stack_level n -∗ ⎡P n⎤ -∗ P.
+Proof.
+  intros; iIntros "#? H".
+  iApply bi.impl_elim_r; iSplit; first iApply "H".
+  by iApply monPred_in_elim.
+Qed.
+
+Lemma stack_level_embed : forall n (P : assert), ⊢ stack_level n -∗ P -∗ ⎡P n⎤.
+Proof.
+  split => ?; rewrite /stack_level; monPred.unseal.
+  iIntros "_" (? [=]); rewrite monPred_at_affinely /=.
+  iIntros ([=] ? [=]); subst; auto.
+Qed.
+
+Lemma stack_level_eq : forall a b, ⊢ stack_level a -∗ stack_level b -∗ ⌜a = b⌝.
+Proof.
+  split => n; rewrite /stack_level; monPred.unseal; setoid_rewrite monPred_at_affinely; simpl.
+  iIntros; iPureIntro; congruence.
+Qed.
+
 Definition env_matches (rho : environ) (ge : genv) (ve : env) (te : temp_env) :=
   (forall i, Genv.find_symbol ge i = lookup i (ge_of rho)) /\
   (forall i, ve !! i = lookup i (ve_of rho)) /\
